TODO.md
@@ -1,5 +1,9 @@
 # TODO
 
+## 2026-07-03
+
+- Tidy up test.lean by using Z.lean
+
 ## 2026-07-02
 
 - Make V_singleton and V_union into the functions. 
